src/LLBC_plus.v
@@ -1,0 +1,211 @@
+Require Import base.
+Require Import lang.
+Require Import List.
+Import ListNotations.
+Require Import PeanoNat Lia.
+(* Notation conflict between stdpp's `+++` and our `+++`. That's why we're importing stpp first,
+   then closing the scope. *)
+From stdpp Require Import pmap gmap.
+Close Scope stdpp_scope.
+Require Import PathToSubtree.
+
+Inductive LLBC_plus_val :=
+| LLBC_plus_bot
+| LLBC_plus_int (n : nat) (* TODO: use Aeneas integer types? *)
+| LLBC_plus_mut_loan (l : loan_id)
+| LLBC_plus_mut_borrow (l : loan_id) (v : LLBC_plus_val)
+(*
+| LLBC_plus_shr_loan (l : loan_id) (v : LLBC_plus_val)
+| LLBC_plus_shr_borrow (l : loan_id)
+ *)
+(* | LLBC_plus_pair (v0 : LLBC_plus_val) (v1 : LLBC_plus_val) *)
+(* Note: symbolic values should be parameterized by a type, when we introduce other datatypes than
+   integers. *)
+| LLBC_plus_symbolic
+.
+
+Variant LLBC_plus_nodes :=
+| LLBC_plus_botC
+| LLBC_plus_intC (n : nat)
+| LLBC_plus_mut_loanC (l : loan_id)
+| LLBC_plus_mut_borrowC (l : loan_id)
+| LLBC_plus_symbolicC
+.
+
+Instance EqDecision_LLBC_plus_nodes : EqDecision LLBC_plus_nodes.
+Proof. unfold RelDecision, Decision. repeat decide equality. Qed.
+
+Definition LLBC_plus_arity c := match c with
+| LLBC_plus_botC => 0
+| LLBC_plus_intC _ => 0
+| LLBC_plus_mut_loanC _ => 0
+| LLBC_plus_mut_borrowC _ => 1
+| LLBC_plus_symbolicC => 0
+end.
+
+Definition LLBC_plus_get_node v := match v with
+| LLBC_plus_bot => LLBC_plus_botC
+| LLBC_plus_int n => LLBC_plus_intC n
+| LLBC_plus_mut_loan l => LLBC_plus_mut_loanC l
+| LLBC_plus_mut_borrow l _ => LLBC_plus_mut_borrowC l
+| LLBC_plus_symbolic => LLBC_plus_symbolicC
+end.
+
+Definition LLBC_plus_children v := match v with
+| LLBC_plus_bot => []
+| LLBC_plus_int _ => []
+| LLBC_plus_mut_loan _ => []
+| LLBC_plus_mut_borrow _ v => [v]
+| LLBC_plus_symbolic => []
+end.
+
+Definition LLBC_plus_fold c vs := match c, vs with
+| LLBC_plus_intC n, [] => LLBC_plus_int n
+| LLBC_plus_mut_loanC l, [] => LLBC_plus_mut_loan l
+| LLBC_plus_mut_borrowC l, [v] => LLBC_plus_mut_borrow l v
+| LLBC_plus_symbolicC, [] => LLBC_plus_symbolic
+| _, _ => LLBC_plus_bot
+end.
+
+Fixpoint LLBC_plus_weight node_weight v :=
+  match v with
+  | LLBC_plus_mut_borrow l v => node_weight (LLBC_plus_mut_borrowC l) + LLBC_plus_weight node_weight v
+  | v => node_weight (LLBC_plus_get_node v)
+end.
+
+Program Instance ValueLLBC_plus : Value LLBC_plus_val LLBC_plus_nodes := {
+  arity := LLBC_plus_arity;
+  get_node := LLBC_plus_get_node;
+  children := LLBC_plus_children;
+  fold_value := LLBC_plus_fold;
+  vweight := LLBC_plus_weight;
+  bot := LLBC_plus_bot;
+}.
+Next Obligation. destruct v; reflexivity. Qed.
+Next Obligation.
+  intros [] [] eq_nodes eq_children; inversion eq_nodes; inversion eq_children; reflexivity.
+Qed.
+Next Obligation.
+  intros [] ? H; (rewrite length_zero_iff_nil in H; rewrite H) ||
+                  destruct (length_1_is_singleton H) as [? ->];
+                  reflexivity.
+Qed.
+Next Obligation.
+  intros [] ? H; (rewrite length_zero_iff_nil in H; rewrite H) ||
+                  destruct (length_1_is_singleton H) as [? ->];
+                  reflexivity.
+Qed.
+Next Obligation. reflexivity. Qed.
+Next Obligation. intros ? []; cbn; lia. Qed.
+
+Record LLBC_plus_state := {
+  vars : Pmap LLBC_plus_val;
+  anons : Pmap LLBC_plus_val;
+  regions : Pmap (Pmap LLBC_plus_val);
+}.
+
+Definition encode_var (x : var) :=
+  encode (A := _ + positive * positive) (inl (encode (A := _ + anon) (inl x))).
+Definition encode_anon (a : anon) :=
+  encode (A := _ + positive * positive) (inl (encode (A := var + _) (inr a))).
+Definition encode_region (x : positive * positive) := encode (A := var + anon + _) (inr x).
+
+(* Collapse the 2-dimensional map of regions into a 1-dimensional map. *)
+Section Flatten.
+  Context {V : Type}.
+
+  Definition flatten : Pmap (Pmap V) -> gmap (positive * positive) V :=
+    map_fold (fun i m Ms => union (kmap (fun j => (i, j)) m) Ms) empty.
+
+  Lemma flatten_insert Ms i m (G : lookup i Ms = None) :
+    flatten (insert i m Ms) = union (kmap (fun j => (i, j)) m) (flatten Ms).
+  Proof.
+    unfold flatten. rewrite map_fold_insert_L.
+    - reflexivity.
+    - intros. rewrite !map_union_assoc. f_equal. apply map_union_comm.
+      apply map_disjoint_spec.
+      intros ? ? ? (? & ? & _)%lookup_kmap_Some (? & ? & _)%lookup_kmap_Some. congruence.
+      all: typeclasses eauto.
+    - assumption.
+  Qed.
+
+  Lemma lookup_None_flatten Ms i j : lookup i Ms = None -> lookup (i, j) (flatten Ms) = None.
+  Proof.
+    intros ?.
+    induction Ms as [ | k x Ms ? _ IHm] using map_first_key_ind.
+    - unfold flatten. rewrite map_fold_empty, lookup_empty. reflexivity.
+    - assert (i <> k). { intros <-. simpl_map. congruence. }
+      simpl_map.
+      rewrite flatten_insert by assumption. apply lookup_union_None_2.
+      + apply eq_None_ne_Some_2.
+        intros ? (? & ? & _)%lookup_kmap_Some; [congruence | typeclasses eauto].
+      + auto.
+  Qed.
+
+  Lemma alter_flatten f i j Ms :
+    alter f (i, j) (flatten Ms) = flatten (alter (alter f j) i Ms).
+  Proof.
+    induction Ms as [ | k x Ms ? _ IHm] using map_first_key_ind.
+    - rewrite !map_alter_not_in_domain by now simpl_map. reflexivity.
+    - destruct (decide (i = k)) as [<- | ].
+      + rewrite alter_insert.
+        rewrite !flatten_insert by assumption.
+        unfold union, map_union. rewrite alter_union_with_l. 
+        * now rewrite kmap_alter by typeclasses eauto.
+        * reflexivity.
+        * intros ? ?. rewrite lookup_None_flatten; easy.
+      + rewrite alter_insert_ne by assumption. rewrite !flatten_insert by now simpl_map.
+        unfold union, map_union. rewrite alter_union_with by reflexivity. rewrite IHm.
+        rewrite map_alter_not_in_domain.
+        * reflexivity.
+        * rewrite eq_None_not_Some.
+          intros (? & ? & _)%lookup_kmap_is_Some; [congruence | typeclasses eauto].
+  Qed.
+End Flatten.
+
+(* TODO: move in base.v *)
+Lemma alter_map_union {V} `{FinMap K M} (m0 m1 : M V) f k :
+  alter f k (union m0 m1) = union (alter f k m0) (alter f k m1).
+Proof.
+  apply map_eq. intros i. destruct (decide (i = k)) as [-> | ].
+  - simpl_map. rewrite !lookup_union. simpl_map.
+Admitted.
+
+Program Instance IsState : State LLBC_plus_state LLBC_plus_val := {
+  extra := unit;
+  get_map S := sum_maps (sum_maps (vars S) (anons S)) (flatten (regions S));
+  get_extra _ := ();
+  alter_at_accessor f a S :=
+    match decode' (A := positive + positive * positive) a with
+    | Some (inl a) =>
+        match decode' (A := var + anon) a with
+        | Some (inl x) => {| vars := alter f x (vars S); anons := anons S; regions := regions S|}
+        | Some (inr a) => {| vars := vars S; anons := alter f a (anons S); regions := regions S|}
+        | None => S
+        end
+    | Some (inr (i, j)) => {| vars := vars S; anons := anons S;
+                              regions := alter (fun r => alter f j r) i (regions S)|}
+    | None => S
+    end;
+  anon_accessor := encode_anon;
+  accessor_anon x :=
+    match decode (A := var + positive) x with
+    | Some (inr a) => Some a
+    | _ => None
+    end;
+  add_anon a v S := {| vars := vars S; anons := insert a v (anons S)|};
+}.
+Next Obligation. reflexivity. Qed.
+Next Obligation.
+  intros ? ? y. cbn. destruct (decode' y) as [[z | (i & j)] | ] eqn:H.
+  - rewrite decode'_is_Some in H.
+    destruct (decode' z) as [[x | a] | ] eqn:G.
+    + cbn. rewrite decode'_is_Some in G. rewrite <-H, <-G, <- !sum_maps_alter_inl.
+      reflexivity.
+    + cbn. rewrite decode'_is_Some in G.
+      rewrite <-H, <-G, <-sum_maps_alter_inr, <-sum_maps_alter_inl. reflexivity.
+    + symmetry. apply map_alter_not_in_domain. rewrite <-H, sum_maps_lookup_l.
+      now apply sum_maps_lookup_None.
+  - cbn. rewrite decode'_is_Some in H. rewrite <-H,  sum_maps_alter_inr, alter_flatten. reflexivity.
+  - symmetry. apply map_alter_not_in_domain, sum_maps_lookup_None. assumption.
+Qed.
